examples and not doing things backwards

SSA/Examples/InstCombinePeepholeRewrites.lean
@@ -17,78 +17,98 @@ register_simp_attr outUserType
 register_simp_attr BitVector.width
 register_simp_attr uncurry
 
-example : TSSA Op ∅ (TSSAIndex.REGION (.base (BaseType.bitvec 32)) (.base (.bitvec 32))) := 
+def thingy : TSSA Op ∅ (TSSAIndex.REGION (.base (BaseType.bitvec 32)) (.base (.bitvec 32))) := 
   TSSA.rgn (arg := 'x'.toNat) <|
   TSSA.ret 
-    (TSSA.assign 'a'.toNat (TSSA.pair Context.Var.first Context.Var.first) <|
-      TSSA.assign 'y'.toNat 
-      (TSSA.op (Op.and 32) Context.Var.first TSSA.rgn0) <|
-     TSSA.assign 'b'.toNat (TSSA.pair Context.Var.first 
-       (Context.Var.next <| Context.Var.next <| Context.Var.first)) <|
-     TSSA.assign 'z'.toNat 
-       (TSSA.op (Op.or 32) Context.Var.first TSSA.rgn0) <|
-     TSSA.nop) 
-    (Context.Var.next <| Context.Var.next <| Context.Var.next <| 
-      Context.Var.first)
+    (TSSA.assign (TSSA.assign (TSSA.assign (TSSA.assign TSSA.nop 
+      'a'.toNat (TSSA.pair Context.Var.last Context.Var.last)) 
+      'y'.toNat (TSSA.op (Op.and 32) Context.Var.last TSSA.rgn0)) 
+      'b'.toNat (TSSA.pair Context.Var.last Context.Var.last.prev.prev)) 
+      'z'.toNat (TSSA.op (Op.or 32) Context.Var.last TSSA.rgn0)) 
+    Context.Var.last
+
+
+example : thingy.eval = sorry := by
+  simp [TypedUserSemantics.eval, UserType.mkPair]
+  admit
+
+def thingy2 : TSSA Op 
+  ((Context.empty.snoc 'x'.toNat (.base $ .bitvec 32)).snoc 
+    'Α'.toNat (.base $ .bitvec 16)) 
+  (.TERMINATOR (.base $ .bitvec 32)) := 
+  TSSA.ret 
+    (TSSA.assign (TSSA.assign (TSSA.assign (TSSA.assign (TSSA.assign
+      TSSA.nop 
+      'a'.toNat (TSSA.pair Context.Var.last.prev Context.Var.last.prev)) 
+      'y'.toNat (TSSA.op (Op.and 32) Context.Var.last TSSA.rgn0)) 
+      'b'.toNat (TSSA.pair Context.Var.last Context.Var.last.prev.prev.prev))
+      'c'.toNat (TSSA.pair Context.Var.last Context.Var.last.prev.prev.prev))
+      'z'.toNat (TSSA.op (Op.or 32) Context.Var.last.prev TSSA.rgn0))
+    Context.Var.last
+
+example : thingy2.eval = sorry := by
+  simp [TypedUserSemantics.eval, UserType.mkPair]
+  admit
 
 theorem Option.some_eq_pure {α : Type u} : @some α = @pure _ _ _ := rfl
-
-theorem InstCombineShift279 : ∀ w : ℕ+, ∀ C : BitVector w,
-  let minus_one : BitVector w := (-1).toBitVector
-  let Γ : Context UserType := List.toAList [⟨42, .unit⟩]
-  ∀ (e : EnvC Γ),  -- for metavariable in typeclass
-  --@SSA.teval BaseType instDecidableEqBaseType instGoedelBaseType SSAIndex.REGION Op TUS
-  SSA.teval e.toEnvU [dsl_region| dsl_rgn %v0  =>
-    %v42 := unit: ;
-    %v1 := op: const C %v42;
-    %v2 := pair: %v0 %v1;
-    %v3 := op: lshr w %v2;
-    %v4 := pair: %v3 %v1;
-    %v5 := op: shl w %v4
-    dsl_ret %v5] (SSA.UserType.base (BaseType.bitvec w))
-    (SSA.UserType.base (BaseType.bitvec w)) =
-  SSA.teval e.toEnvU [dsl_region| dsl_rgn %v0 =>
-    %v42 := unit: ;
-    %v1 := op: const minus_one %v42;
-    %v2 := op: const C %v42;
-    %v3 := pair: %v1 %v2;
-    %v4 := op: shl w %v3;
-    %v5 := pair: %v0 %v4;
-    %v6 := op: and w %v5
-    dsl_ret %v6] (SSA.UserType.base (BaseType.bitvec w))
-    (SSA.UserType.base (BaseType.bitvec w)) := by
-      intros w C minus_one Γ e
-      funext x
-      simp only [SSA.teval]
-      simp only [Function.comp]
-      simp only [id.def]
-      simp only [SSA.teval]
-      simp only [EnvU.set]
-      simp only [if_false]
-      simp only [if_true]
-      simp only [TypedUserSemantics.outUserType]
-      simp only [TypedUserSemantics.argUserType]
-      simp only [TypedUserSemantics.rgnDom]
-      simp only [TypedUserSemantics.rgnCod]
-      simp only [TypedUserSemantics.eval]
-      simp only [outUserType]
-      simp only [eval]
-      simp only [if_true]
-      simp only [argUserType]
-      simp only [Option.some_eq_pure]
-      simp only [EnvC.toEnvU]
-      simp only [uncurry]
-      simp only [Option.elim]
-      simp only [BitVector.width]
-      simp only [pure_bind]
-      simp only [dite_true]
-      simp only [pure_bind]
-      simp only [dite_true]
-      simp only [pure_bind]
-      simp only [dite_true]
-      simp only [pure_bind]
-      simp only [if_true]
-      simp only [pure_bind]
-      simp only [dite_true]
-      congr
-      rw [InstCombineShift279_base]
+-- @Goens fix this
+-- @bollu fix notation
+-- theorem InstCombineShift279 : ∀ w : ℕ+, ∀ C : BitVector w,
+--   let minus_one : BitVector w := (-1).toBitVector
+--   let Γ : Context UserType := List.toAList [⟨42, .unit⟩]
+--   ∀ (e : EnvC Γ),  -- for metavariable in typeclass
+--   --@SSA.teval BaseType instDecidableEqBaseType instGoedelBaseType SSAIndex.REGION Op TUS
+--   SSA.teval e.toEnvU [dsl_region| dsl_rgn %v0  =>
+--     %v42 := unit: ;
+--     %v1 := op: const C %v42;
+--     %v2 := pair: %v0 %v1;
+--     %v3 := op: lshr w %v2;
+--     %v4 := pair: %v3 %v1;
+--     %v5 := op: shl w %v4
+--     dsl_ret %v5] (SSA.UserType.base (BaseType.bitvec w))
+--     (SSA.UserType.base (BaseType.bitvec w)) =
+--   SSA.teval e.toEnvU [dsl_region| dsl_rgn %v0 =>
+--     %v42 := unit: ;
+--     %v1 := op: const minus_one %v42;
+--     %v2 := op: const C %v42;
+--     %v3 := pair: %v1 %v2;
+--     %v4 := op: shl w %v3;
+--     %v5 := pair: %v0 %v4;
+--     %v6 := op: and w %v5
+--     dsl_ret %v6] (SSA.UserType.base (BaseType.bitvec w))
+--     (SSA.UserType.base (BaseType.bitvec w)) := by
+--       intros w C minus_one Γ e
+--       funext x
+--       simp only [SSA.teval]
+--       simp only [Function.comp]
+--       simp only [id.def]
+--       simp only [SSA.teval]
+--       simp only [EnvU.set]
+--       simp only [if_false]
+--       simp only [if_true]
+--       simp only [TypedUserSemantics.outUserType]
+--       simp only [TypedUserSemantics.argUserType]
+--       simp only [TypedUserSemantics.rgnDom]
+--       simp only [TypedUserSemantics.rgnCod]
+--       simp only [TypedUserSemantics.eval]
+--       simp only [outUserType]
+--       simp only [eval]
+--       simp only [if_true]
+--       simp only [argUserType]
+--       simp only [Option.some_eq_pure]
+--       simp only [EnvC.toEnvU]
+--       simp only [uncurry]
+--       simp only [Option.elim]
+--       simp only [BitVector.width]
+--       simp only [pure_bind]
+--       simp only [dite_true]
+--       simp only [pure_bind]
+--       simp only [dite_true]
+--       simp only [pure_bind]
+--       simp only [dite_true]
+--       simp only [pure_bind]
+--       simp only [if_true]
+--       simp only [pure_bind]
+--       simp only [dite_true]
+--       congr
+--       rw [InstCombineShift279_base]
